ulib/FStar.Bytes.fst
@@ -3,8 +3,7 @@ type byte = FStar.UInt8.byte
 
 open FStar.All
 
-assume type bytes
-assume HasEq_bytes: hasEq bytes
+assume type bytes : eqtype
 
 assume val length : bytes -> Tot nat
 assume val get : b:bytes -> pos:nat{pos < length b} -> Tot byte
