ulib/FStar.Constructive.fst
@@ -26,7 +26,7 @@ type ceq_type (a:Type) : Type -> Type =
 val eq_ind : #a:Type -> x:a -> p:(a -> Type) -> f:p x -> y:a -> e:ceq x y -> Tot (p y)
 let eq_ind #a x p f y _ = f
 
-val ceq_eq : #a:Type{hasEq a} -> #x:a -> #y:a -> h:(ceq x y) -> Lemma (x = y)
+val ceq_eq : #a:eqtype -> #x:a -> #y:a -> h:(ceq x y) -> Lemma (x = y)
 let ceq_eq #a #x #y h = ()
 
 val ceq_congruence : #a:Type -> #b:Type -> #x:a -> #y:a -> ceq x y ->
