ulib/FStar.Monotonic.RRef.fst
@@ -27,16 +27,7 @@ type rid = r:HH.rid{is_eternal_region r}
  *)
 abstract type m_rref (r:rid) (a:Type) (b:reln a) = x:HS.ref a{x.id = r}
 
-(* let haseq_m_rref (r:rid) (a:Type) (b:reln a)  *)
-(*     : Lemma (requires True) *)
-(* 	    (ensures (hasEq (m_rref r a b))) *)
-(* 	    [SMTPat (hasEq (m_rref r a b))] *)
-(*     = () *)
 
-(* val as_rref: #r:rid -> #a:Type -> #b:reln a -> m_rref r a b -> GTot (rref r a) *)
-(* let as_rref #r #a #b x = x *)
-
-(* assume HasEq_m_rref: forall (r:rid) (a:Type) (b:reln a).{:pattern (hasEq (m_rref r a b))} hasEq (m_rref r a b) *)
 (*
  * AR: the refinement is important here, for as_rref rid was part of the type index
  *)
